主要还是利用了倍角公式

$\sin(\alpha+\beta)=\sin(\alpha)\cos(\beta)+\cos(\alpha)\sin(\beta)$      (1)​

$\sin(\alpha-\beta)=\sin(\alpha)\cos(\beta)-\cos(\alpha)\sin(\beta)$      (2)

$\cos(\alpha+\beta)=\cos(\alpha)\cos(\beta)-\sin(\alpha)\sin(\beta)$      (3)

$\cos(\alpha-\beta)=\cos(\alpha)\cos(\beta)+\sin(\alpha)\sin(\beta)$      (4)

(1) + (2): $\sin(\alpha+\beta)+\sin(\alpha-\beta)=2\sin(\alpha)\cos(\beta)$     (5)

(a). $\sin(\alpha)\cos(\beta)=\frac{\sin(\alpha+\beta)+\sin(\alpha-\beta)}{2}$   即 “积化和差”

(b). 在 (5) 中，令 $\alpha=\frac{x+y}{2}, \beta=\frac{x-y}{2}$, 即 $\alpha + \beta = x, \alpha-\beta=y$,   可得：$\sin(x)+\sin(y)=2\sin(\frac{x+y}{2})\cos(\frac{x-y}{2})$

其余的推导类似。

